\documentclass{article}
\usepackage{amsmath} % For mathematical symbols and align environment
\usepackage{amssymb} % For additional symbols

\begin{document}

\section*{Question A2}
\subsection*{(a)}

\quad Since $\mathbb{E}[Y] = \mathbb{E}[\mathbb{E}[Y \mid X]]$ (by the Law of Total Expectation), we know:
\[
    \mathbb{E}[Y \mid X] = X \implies \mathbb{E}[Y] = \mathbb{E}[X].
\]

By the definition of covariance:
\[
    \text{Cov}(X, Y) = \mathbb{E}[(X - \mathbb{E}[X])(Y - \mathbb{E}[Y])].
\]

Expanding this out:
\[
    \text{Cov}(X, Y) = \mathbb{E}[XY] - \mathbb{E}[X] \cdot \mathbb{E}[Y].
\]

Substituting $\mathbb{E}[Y \mid X] = X$, we get:
\[
    \text{Cov}(X, Y) = \mathbb{E}[X \cdot X] - \mathbb{E}[X] \cdot \mathbb{E}[X].
\]

This simplifies to:
\[
    \text{Cov}(X, Y) = \mathbb{E}[X^2] - (\mathbb{E}[X])^2.
\]

Now, using the expansion:
\[
    \mathbb{E}[X^2] - (\mathbb{E}[X])^2 = \mathbb{E}[(X - \mathbb{E}[X])^2].
\]

Thus:
\[
    \text{Cov}(X, Y) = \mathbb{E}[(X - \mathbb{E}[X])^2].
\]

\hfill\(\blacksquare\)

\end{document}
