\documentclass{article}
\usepackage{amsmath} % For mathematical symbols and align environment
\usepackage{amssymb} % For additional symbols

\begin{document}

\section*{Question A2}
\subsection*{(b)}

We know that $\text{Cov}(X, Y) = \mathbb{E}[XY] - \mathbb{E}[X] \cdot \mathbb{E}[Y]$. To show $\text{Cov}(X, Y) = 0$, we need to prove:
\[
\mathbb{E}[XY] = \mathbb{E}[X] \cdot \mathbb{E}[Y].
\]

By the definition of expectation of the joint PDF:
\[
\mathbb{E}[XY] = \int_{-\infty}^\infty \int_{-\infty}^\infty xy f_{X,Y}(x, y) \, dx \, dy.
\]

Using independence:
\[
f_{X,Y}(x, y) = f_X(x) f_Y(y).
\]

Substituting this into the expression for $\mathbb{E}[XY]$, we have:
\[
\mathbb{E}[XY] = \int_{-\infty}^\infty \int_{-\infty}^\infty xy f_X(x) f_Y(y) \, dx \, dy.
\]

The double integral can be separated:
\[
\mathbb{E}[XY] = \left( \int_{-\infty}^\infty x f_X(x) \, dx \right) \cdot \left( \int_{-\infty}^\infty y f_Y(y) \, dy \right).
\]

The first term is $\mathbb{E}[X]$, and the second term is $\mathbb{E}[Y]$. Thus:
\[
\mathbb{E}[XY] = \mathbb{E}[X] \cdot \mathbb{E}[Y].
\]

Therefore:
\[
\text{Cov}(X, Y) = \mathbb{E}[XY] - \mathbb{E}[X] \cdot \mathbb{E}[Y] = 0.
\]

\hfill\(\blacksquare\)

\end{document}
