\documentclass{article}
\usepackage{amsmath} % For mathematical symbols and align environment
\usepackage{amssymb} % For additional symbols

\begin{document}

\section*{A3(b)}

We proved in (a) that:
\[
h(z) = \int_{-\infty}^\infty f(x) g(z - x) \, dx.
\]

Since \( f \) and \( g \) are nonzero only on \([0,1]\), we note that \( g(z - x) \) is:
\[
g(z - x) =
\begin{cases}
1 & \text{for } 0 \leq z - x \leq 1, \\
0 & \text{otherwise.}
\end{cases}
\]

Plugging in values:
\[
h(z) = \int_0^1 g(z - x) \, dx.
\]

For \( 0 \leq z \leq 1 \), \( g(z - x) = 1 \) for \( x \in [0, z] \):
\[
h(z) = \int_0^z 1 \, dx = z.
\]

For \( 1 < z \leq 2 \), \( g(z - x) = 1 \) for \( x \in [z - 1, 1] \):
\[
h(z) = \int_{z-1}^1 1 \, dx = 1 - (z - 1) = 2 - z.
\]

Thus:
\[
h(z) =
\begin{cases}
z & \text{for } 0 \leq z \leq 1, \\
2 - z & \text{for } 1 < z \leq 2, \\
0 & \text{otherwise.}
\end{cases}
\]

\hfill\(\blacksquare\)

\end{document}
