\documentclass{article}
\usepackage{amsmath} % For mathematical symbols and align environment
\usepackage{amssymb} % For additional symbols

\begin{document}

\section*{A4(c)}

\subsection*{Mean}
First, consider the expectation of \( \hat{\mu}_n \):
\[
\mathbb{E}[\hat{\mu}_n] = \mathbb{E} \left[ \frac{1}{n} \sum_{i=1}^n X_i \right] = \frac{1}{n} \sum_{i=1}^n \mathbb{E}[X_i].
\]
Since \( \mathbb{E}[X_i] = \mu \) for all \( i \), this simplifies to:
\[
\mathbb{E}[\hat{\mu}_n] = \frac{1}{n} \cdot n \cdot \mu = \mu.
\]

Now, compute the expectation of \( \sqrt{n} (\hat{\mu}_n - \mu) \):
\[
\mathbb{E}[\sqrt{n} (\hat{\mu}_n - \mu)] = \sqrt{n} \cdot \mathbb{E}[\hat{\mu}_n - \mu].
\]
Substituting \( \mathbb{E}[\hat{\mu}_n] = \mu \), we get:
\[
\mathbb{E}[\sqrt{n} (\hat{\mu}_n - \mu)] = \sqrt{n} \cdot (\mathbb{E}[\hat{\mu}_n] - \mu) = \sqrt{n} \cdot (\mu - \mu) = 0.
\]

\subsection*{Variance}
The variance of \( \sqrt{n} (\hat{\mu}_n - \mu) \) is:
\[
\text{Var}\left(\sqrt{n} (\hat{\mu}_n - \mu)\right) = \text{Var}\left(\sqrt{n} \cdot \frac{1}{n} \sum_{i=1}^n (X_i - \mu)\right).
\]
Simplify the scaling factor \( \sqrt{n} \cdot \frac{1}{n} = \frac{1}{\sqrt{n}} \):
\[
\text{Var}\left(\sqrt{n} (\hat{\mu}_n - \mu)\right) = \frac{1}{n} \cdot \text{Var}\left(\sum_{i=1}^n (X_i - \mu)\right).
\]

Since \( X_1, X_2, \ldots, X_n \) are independent, the variance of the sum is the sum of variances:
\[
\text{Var}\left(\sum_{i=1}^n (X_i - \mu)\right) = \sum_{i=1}^n \text{Var}(X_i - \mu).
\]
Since \( \text{Var}(X_i - \mu) = \text{Var}(X_i) = \sigma^2 \) for all \( i \), this becomes:
\[
\text{Var}\left(\sum_{i=1}^n (X_i - \mu)\right) = n \cdot \sigma^2.
\]

Substitute this back:
\[
\text{Var}\left(\sqrt{n} (\hat{\mu}_n - \mu)\right) = \frac{1}{n} \cdot n \cdot \sigma^2 = \sigma^2.
\]

\subsection*{Final Results}
\begin{itemize}
    \item \textbf{Mean:}
    \[
    \mathbb{E}[\sqrt{n} (\hat{\mu}_n - \mu)] = 0.
    \]
    \item \textbf{Variance:}
    \[
    \text{Var}[\sqrt{n} (\hat{\mu}_n - \mu)] = \sigma^2.
    \]
\end{itemize}

\hfill\(\blacksquare\)

\end{document}
